almost got a version of bind_satisfies_bind that works, except we need to prove some sort of equivalence to replace observing that works...

coq/handwritten/CryptolToCoq/CompM_ITrees.v
@@ -19,159 +19,213 @@ Arguments Spec_exists {E A}.
 (* An ITree that defines a set of ITrees *)
 Definition itree_spec E A : Type := itree (SpecEvent E) A.
 
+(* The body of an itree_spec, inside the observe projection *)
+Definition itree_spec' E A : Type := itree' (SpecEvent E) A.
+
 Variant satisfiesF {E A} (satisfies : itree_spec E A -> itree E A -> Prop)
-  : itree_spec E A -> itree E A -> Prop :=
-| Satisfies_Ret a : satisfiesF satisfies (Ret a) (Ret a)
+  : itree_spec' E A -> itree' E A -> Prop :=
+| Satisfies_Ret a : satisfiesF satisfies (RetF a) (RetF a)
 | Satisfies_TauL spec tree :
-    satisfies spec tree -> satisfiesF satisfies (Tau spec) tree
+    satisfies spec tree ->
+    satisfiesF satisfies (TauF spec) (observe tree)
 | Satisfies_TauR spec tree :
-    satisfies spec tree -> satisfiesF satisfies spec (Tau tree)
+    satisfies spec tree ->
+    satisfiesF satisfies (observe spec) (TauF tree)
 | Satisfies_Vis X (e:E X) spec tree :
     (forall x, satisfies (spec x) (tree x)) ->
-    satisfiesF satisfies (Vis (Spec_vis e) spec) (Vis e tree)
+    satisfiesF satisfies (VisF (Spec_vis e) spec) (VisF e tree)
 | Satisfies_Forall X spec tree :
     (forall x:X, satisfies (spec x) tree) ->
-    satisfiesF satisfies (Vis Spec_forall spec) tree
+    satisfiesF satisfies (VisF Spec_forall spec) (observe tree)
 | Satisfies_Exists X spec tree :
     (exists x:X, satisfies (spec x) tree) ->
-    satisfiesF satisfies (Vis Spec_exists spec) tree
+    satisfiesF satisfies (VisF Spec_exists spec) (observe tree)
 .
 
-Definition satisfies {E A} spec tree := paco2 (@satisfiesF E A) bot2 spec tree.
-
-Lemma satisfiesF_mono E A : monotone2 (@satisfiesF E A).
+Instance Proper_satisfies_satisfiesF {E A} :
+  Proper (pointwise_relation _ (pointwise_relation _ Basics.impl) ==>
+          eq ==> eq ==> Basics.impl) (@satisfiesF E A).
 Proof.
-  intros spec tree r1 r2 sats sub12. destruct sats; constructor.
-  { apply sub12. assumption. }
-  { apply sub12. assumption. }
+  intros R1 R2 implR spec1 spec2 e_spec tree1 tree2 e_tree sats.
+  rewrite <- e_spec; rewrite <- e_tree.
+  destruct sats; constructor; intros; try (apply implR; apply H).
+  destruct H as [ x H ]. exists x. apply implR; assumption.
+Qed.
+
+Lemma satisfiesF_mono {E A} (sats1 sats2:itree_spec E A -> itree E A -> Prop)
+         (sub_sats:forall spec tree, sats1 spec tree -> sats2 spec tree) :
+  forall spec tree,
+    satisfiesF sats1 spec tree -> satisfiesF sats2 spec tree.
+Proof.
+  intros.
+  apply (Proper_satisfies_satisfiesF sats1 sats2 sub_sats _ _ eq_refl _ _ eq_refl H).
+Qed.
+
+Definition satisfies_ {E A} satisfies spec tree :=
+  @satisfiesF E A satisfies (observe spec) (observe tree).
+
+
+Lemma satisfies__mono E A : monotone2 (@satisfies_ E A).
+Proof.
+  intros spec tree r1 r2 sats sub12. unfold satisfies_. destruct sats; constructor.
+  { apply sub12; assumption. }
+  { apply sub12; assumption. }
   { intros; apply sub12. apply H. }
   { intros; apply sub12. apply H. }
   { destruct H as [ x H ]. exists x. apply sub12. apply H. }
 Qed.
 
-Hint Resolve satisfiesF_mono : paco.
+Hint Resolve satisfies__mono : paco.
+
+Definition satisfies {E A} spec tree := paco2 (@satisfies_ E A) bot2 spec tree.
+
+Instance Proper_observing_paco2_satisfies_impl E A r :
+  Proper (observing eq ==> observing eq ==> iff) (paco2 (@satisfies_ E A) r).
+Proof.
+  intros spec1 spec2 [ Rspec ] tree1 tree2 [ Rtree ].
+  split; intro; punfold H; pfold; unfold satisfies_;
+    [ rewrite <- Rtree; rewrite <- Rspec | rewrite Rtree; rewrite Rspec ];
+    apply H.
+Qed.
+
+Lemma observing_eta {E A} (tree:itree E A) : observing eq tree (go (observe tree)).
+Proof.
+  constructor. reflexivity.
+Qed.
+
+Lemma observing_fun_eta {E A B} (tree:A -> itree E B) :
+  pointwise_relation A (observing eq) tree (fun x => go (observe (tree x))).
+Proof.
+  intro a. constructor. reflexivity.
+Qed.
+
+
+
+Lemma satisfies_inv_tau_l E A (P:itree_spec E A) m :
+  satisfies (Tau P) m -> satisfies P m.
+Proof.
+  revert P m; pcofix CIH; intros. punfold H0. inversion H0.
+  { rewrite <- (observing_intros _ _ _ H1). pclearbot.
+    eapply paco2_mon_bot; intros; eassumption. }
+  { rewrite <- (observing_intros _ (Tau tree) _ H1). pfold.
+    apply Satisfies_TauR. right. apply CIH. pclearbot. unfold satisfies.
+    rewrite <- (observing_intros _ _ (Tau P) H). assumption. }
+Qed.
+
+(*
+Lemma satisfies_inv_vis_l E A e X (P:X -> itree_spec E A) m :
+  satisfies (Vis e P) m -> exists m', 
+
+Lemma satisfies_eutt_l E A (P1 P2:itree_spec E A) (e: eutt eq P1 P2) :
+  forall m, satisfies P1 m -> satisfies P2 m.
+Proof.
+  revert P1 P2 e; pcofix CIH. intros P1 P2 e.
+  pose (e' := e).
+  punfold e'. inversion e'; intros.
+  { rewrite <- (observing_intros _ (Ret r2) _ H). rewrite <- REL.
+    rewrite (observing_intros _ (Ret r1) _ H0).
+    eapply paco2_mon_bot; intros; eassumption. }
+  { rewrite <- (observing_intros _ (Tau m2) _ H). pfold.
+    apply Satisfies_TauL. right. apply (CIH m1).
+    - pclearbot. apply REL.
+    - unfold satisfies in H1. rewrite <- (observing_intros _ (Tau m1) _ H0) in H1.
+      apply satisfies_inv_tau_l. apply H1. }
+  { unfold satisfies in H1. rewrite <- (observing_intros _ (Vis e0 k1) _ H0) in H1.
+    punfold H1. inversion H1.
+    - rewrite <- (observing_intros _ (Tau tree) _ H3).
+      rewrite <- (observing_intros _ (Vis e0 k2) _ H).
+      pfold. apply Satisfies_TauR.
+      pclearbot. left.
+
+      rewrite (observing_intros _ (Vis e0 k2) _ H)
+
+
+rewrite <- (observing_intros _ (Vis e0 k2) _ H).
+    - rewrite <- (observing_intros _ (Tau tree) _ H3).
+    apply Satisfies
+
+
+Lemma satisfies_eutt_l' E A (P1 P2:itree_spec' E A)
+      (e: eqitF eq true true id (eutt eq) P1 P2) :
+  forall m, satisfies (go P1) m -> satisfies (go P2) m.
+Proof.
+  revert P1 P2 e; pcofix CIH. intros P1 P2 e m sats. induction e.
+  { rewrite <- REL. eapply paco2_mon_bot; [ eassumption | intros; assumption ]. }
+  { pfold. apply Satisfies_TauL. right. apply CIH.
+FIXME: can't apply CIH, because the argument to Tau is not of the form (go _)
+
+punfold sats. inversion sats.
+*)
+
+Instance Proper_eutt_satisfies E A : Proper (eutt eq ==> eutt eq ==> iff) (@satisfies E A).
+Admitted.
 
 (* The proposition that a is returned by an itree along some path *)
-Inductive is_itree_retval {E A} : itree E A -> A -> Prop :=
-| iirv_ret a : is_itree_retval (Ret a) a
-| iirv_tau itree a : is_itree_retval itree a -> is_itree_retval (Tau itree) a
-| iirv_vis {X} (ev:E X) itree a x : is_itree_retval (itree x) a ->
-                                    is_itree_retval (Vis ev itree) a
+Inductive is_itree_retval' {E A} : itree' E A -> A -> Prop :=
+| iirv_ret a : is_itree_retval' (RetF a) a
+| iirv_tau tree a :
+    is_itree_retval' (observe tree) a -> is_itree_retval' (TauF tree) a
+| iirv_vis {X} (ev:E X) tree a x :
+    is_itree_retval' (observe (tree x)) a ->
+    is_itree_retval' (VisF ev tree) a
 .
+
+Definition is_itree_retval {E A} tree a := @is_itree_retval' E A (observe tree) a.
+
 
 Infix ">>=" := ITree.bind (at level 58, left associativity).
 Notation "m1 >> m2" := (m1 >>= fun _ => m2) (at level 58, left associativity).
 
-Lemma satisfies_untau_l' E A spec tree (sats:@satisfies E A spec tree) spec' :
-  spec = Tau spec' -> satisfies spec' tree.
-Proof.
-  revert spec tree sats spec'; pcofix CIH; intros.
-  punfold sats. destruct sats; try discriminate.
-  - injection H0; intro e; rewrite <- e.
-    pclearbot.
-    eapply paco2_mon_bot; [ eassumption | intros; assumption ].
-  - pfold. apply Satisfies_TauR. pclearbot. right.
-    apply (CIH _ _ H). assumption.
-Qed.
 
-Lemma satisfies_untau_l E A spec tree :
-  @satisfies E A (Tau spec) tree ->
-  satisfies spec tree.
-Proof.
-  intros sats. apply (satisfies_untau_l' E A _ _ sats _ eq_refl).
-Qed.
-
-Lemma satisfies_untau_r' E A spec tree (sats:@satisfies E A spec tree) tree' :
-  tree = Tau tree' -> satisfies spec tree'.
-Proof.
-  revert spec tree sats tree'; pcofix CIH; intros.
-  punfold sats. destruct sats; try discriminate.
-  - pfold. apply Satisfies_TauL. right. pclearbot. apply (CIH _ _ H). assumption.
-  - injection H0; intro e. rewrite <- e. pclearbot.
-    eapply paco2_mon_bot; [ eassumption | intros; assumption ].
-  - pfold. apply Satisfies_Forall; intro. right.
-    pclearbot. apply (CIH _ _ (H x)). assumption.
-  - destruct H as [ x H ]. pfold. apply Satisfies_Exists. exists x.
-    pclearbot. right. apply (CIH _ _ H). assumption.
-Qed.
-
-Lemma satisfies_untau_r E A spec tree :
-  @satisfies E A spec (Tau tree) ->
-  satisfies spec tree.
-Proof.
-  intros sats. apply (satisfies_untau_r' E A _ _ sats _ eq_refl).
-Qed.
-
-Lemma satisfies_eutt_l E A spec tree (sats:@satisfies E A spec tree)
-           spec' (e:eutt eq spec spec') :
-  satisfies spec' tree.
-Proof.
-  (*
-  revert spec tree sats spec' e; pcofix CIH; intros.
-  punfold e. unfold eqit_ in e. rewrite itree_eta.
-  destruct e.
-  { unfold satisfies in sats.
-    eapply paco2_mon_bot; [ eassumption | ].
-  destruct e.
-   *)
-Admitted.
-
-Lemma satisfies_eutt_r E A spec tree
-           (sats:@satisfies E A spec tree)
-           tree' (e:eutt eq tree tree') :
-  satisfies spec tree'.
+(* FIXME: this is not actually true! *)
+Instance Proper_observing_TauF E A : Proper (observing eq ==> eq)
+                                            (TauF (E:=E) (R:=A) (itree:=itree E A)).
 Proof.
 Admitted.
 
-Instance Proper_eutt_satisfies_impl E A :
-  Proper (eutt eq ==> eutt eq ==> iff) (@satisfies E A).
-Proof.
-  intros spec1 spec2 e_spec tree1 tree2 e_tree.
-  split; intro H.
-  - eapply satisfies_eutt_l; [ | eassumption ].
-    eapply satisfies_eutt_r; [ | eassumption ].
-    assumption.
-  - eapply satisfies_eutt_l; [ | symmetry; eassumption ].
-    eapply satisfies_eutt_r; [ | symmetry; eassumption ].
-    assumption.
-Qed.
-
-(*
-Instance Proper_eutt_paco2_satisfies_impl E A r :
-  Proper (eutt eq ==> eutt eq ==> iff) (paco2 (@satisfiesF E A) r).
+(* FIXME: this is not actually true! *)
+Instance Proper_observing_VisF E A X :
+  Proper (eq ==> pointwise_relation X (observing eq) ==> eq)
+         (VisF (E:=E) (R:=A) (itree:=itree E A) (X:=X)).
 Proof.
 Admitted.
-*)
 
-Instance Proper_observing_paco2_satisfies_impl E A r :
-  Proper (observing eq ==> observing eq ==> iff) (paco2 (@satisfiesF E A) r).
-Proof.
-  intros spec1 spec2 [ Rspec ] tree1 tree2 [ Rtree ]. split; intro.
-Admitted.
-
-Lemma bind_satisfies_bind E A B (P:itree_spec E A) (Q:A -> itree_spec E B)
-      (m:itree E A) (f:A -> itree E B) :
-  satisfies P m ->
-  (forall a, is_itree_retval m a -> satisfies (Q a) (f a)) ->
-  satisfies (P >>= Q) (m >>= f).
+Lemma bind_satisfies_bind' E A B (P:itree_spec' E A) (Q:A -> itree_spec E B)
+      (m:itree' E A) (f:A -> itree E B) :
+  satisfiesF satisfies P m ->
+  (forall a, is_itree_retval' m a -> satisfies (Q a) (f a)) ->
+  satisfies (go P >>= Q) (go m >>= f).
 Proof.
   intro sats; revert P m sats. pcofix CIH.
-  intros P m sats; punfold sats; destruct sats; intros.
-  { eapply paco2_mon_bot; [ |  intros; eassumption ].
-    rewrite bind_ret_. rewrite bind_ret_. apply H0. constructor. }
-  { rewrite bind_tau_. pfold. apply Satisfies_TauL. pclearbot. right.
-    apply CIH; assumption. }
-  { rewrite bind_tau_. pfold. apply Satisfies_TauR. pclearbot. right.
-    apply CIH; [ assumption | ]. intros. apply H0. apply iirv_tau; assumption. }
-  { rewrite bind_vis_. rewrite bind_vis_. pfold. pclearbot.
-    apply Satisfies_Vis. intro. right. apply CIH; [ apply H | ].
-    intros a iirv. apply H0.
-    apply (iirv_vis _ _ _ x). assumption. }
-  { rewrite bind_vis_. pfold. pclearbot. apply Satisfies_Forall. intros. right.
-    apply CIH; [ apply (H x) | apply H0 ]. }
-  { rewrite bind_vis_. pfold. pclearbot. apply Satisfies_Exists.
-    destruct H as [ x H ]. exists x. right. pclearbot.
-    apply CIH; [ apply H | apply H0 ]. }
+  intros P m sats; destruct sats; intros.
+  { repeat rewrite bind_ret_. eapply paco2_mon_bot; [ | intros; eassumption ].
+    apply H0. constructor. }
+  { rewrite (observing_eta spec). rewrite bind_tau_. pfold. apply Satisfies_TauL. right.
+    apply CIH; [ | apply H0 ]. punfold H. unfold satisfies_ in H.
+    eapply satisfiesF_mono; [ | eassumption ].
+    intros s t sats. pclearbot. apply sats. }
+  { rewrite (observing_eta tree). rewrite bind_tau_. pfold. apply Satisfies_TauR. right.
+    apply CIH.
+    - punfold H. eapply satisfiesF_mono; [ | eassumption ].
+      intros. pclearbot. assumption.
+    - intros. apply H0. apply iirv_tau; assumption. }
+  { rewrite (observing_fun_eta spec). rewrite (observing_fun_eta tree).
+    rewrite bind_vis_. rewrite bind_vis_. pfold.
+    apply Satisfies_Vis. intro. right. apply CIH.
+    - pose (sats := H x). punfold sats. eapply satisfiesF_mono; [ | eassumption ].
+      intros; pclearbot; assumption.
+    - intros; apply H0. eapply iirv_vis. eassumption. }
+  { rewrite (observing_fun_eta spec). rewrite bind_vis_. pfold.
+    apply Satisfies_Forall. intros. right.
+    apply CIH; [ | apply H0 ].
+    pose (sats := H x). punfold sats. eapply satisfiesF_mono; [ | eassumption ].
+    intros. pclearbot. assumption. }
+  { rewrite (observing_fun_eta spec). rewrite bind_vis_. pfold.
+    apply Satisfies_Exists.
+    destruct H as [ x sats ]. exists x. right.
+    apply CIH; [ | apply H0 ].
+    punfold sats. eapply satisfiesF_mono; [ | eassumption ].
+    intros. pclearbot. assumption. }
 Qed.
 
 
